add counters for min, max size bounds

src/cddl/pulse/CDDL.Pulse.Serialize.Gen.MapGroup.ZeroOrMore.Aux2.Invariant.fst
@@ -50,6 +50,23 @@ let impl_serialize_map_zero_or_more_iterator_gen_invariant_min
     )
   )
 
+let impl_serialize_map_zero_or_more_iterator_gen_update_min
+  (#pe: cbor_parser)
+  (minl: (cbor_min_length pe))
+  (#key: typ) (#tkey: Type0)
+  (sp1: (spec key tkey true))
+  (#value: typ) (#tvalue: Type0)
+  (#inj: bool)
+  (sp2: (spec value tvalue inj))
+  (except: map_constraint { inj \/ map_constraint_value_injective key sp2.parser except })
+  (n: nat)
+  (k: tkey)
+  (v: tvalue)
+: Tot nat
+= if sp1.serializable k && sp2.serializable v
+  then n + minl (sp1.serializer k) + minl (sp2.serializer v)
+  else 0 (* dummy *)
+
 let impl_serialize_map_zero_or_more_iterator_gen_invariant_max
   (#pe: cbor_parser)
   (#minl: (cbor_min_length pe))
@@ -78,6 +95,30 @@ let impl_serialize_map_zero_or_more_iterator_gen_invariant_max
     )
   )
 
+let impl_serialize_map_zero_or_more_iterator_gen_update_max
+  (#pe: cbor_parser)
+  (maxl: (cbor_max_length pe))
+  (#key: typ) (#tkey: Type0)
+  (sp1: (spec key tkey true))
+  (#value: typ) (#tvalue: Type0)
+  (#inj: bool)
+  (sp2: (spec value tvalue inj))
+  (except: map_constraint { inj \/ map_constraint_value_injective key sp2.parser except })
+  (n: option nat)
+  (k: tkey)
+  (v: tvalue)
+: Tot (option nat)
+= match n with
+  | None -> None
+  | Some n' ->
+    if sp1.serializable k && sp2.serializable v
+    then match maxl (sp1.serializer k) with
+    | None -> None
+    | Some n1 ->
+      match maxl (sp2.serializer v) with
+      | None -> None
+      | Some n2 -> Some (n' + n1 + n2)
+    else None (* dummy *)
 
 let impl_serialize_map_zero_or_more_iterator_gen_invariant0
   (#pe: cbor_parser)
@@ -106,20 +147,54 @@ let impl_serialize_map_zero_or_more_iterator_gen_invariant0
         )
       )
 
-let impl_serialize_map_zero_or_more_iterator_gen_invariant
+let impl_serialize_map_zero_or_more_iterator_gen_invariant1
   (#pe: cbor_parser)
   (#minl: (cbor_min_length pe))
   (#maxl: (cbor_max_length pe))
-  (#tkey: Type)
-  (#tvalue: Type)
   (p: (cbor_map_parser minl maxl))
+  (#key: typ) (#tkey: Type0)
+  (sp1: (spec key tkey true))
+  (#value: typ) (#tvalue: Type0)
+  (#inj: bool)
+  (sp2: (spec value tvalue inj))
+  (except: map_constraint { inj \/ map_constraint_value_injective key sp2.parser except })
   (em: bool)
   (out: S.slice U8.t)
   (vout: Seq.seq U8.t)
   (size: SZ.t)
   (count: U64.t)
   (m: cbor_map)
+  (v0: Map.t tkey (list tvalue))
   (v: Map.t tkey (list tvalue))
+  (min: nat)
+  (max: option nat)
   (res: bool)
 : prop
-= impl_serialize_map_zero_or_more_iterator_gen_invariant0 p em out vout size count m v res
+= impl_serialize_map_zero_or_more_iterator_gen_invariant0 p em out vout size count m v res /\
+  impl_serialize_map_zero_or_more_iterator_gen_invariant_min p sp1 sp2 except min v0 v /\
+  impl_serialize_map_zero_or_more_iterator_gen_invariant_max p sp1 sp2 except max v0 v 
+
+let impl_serialize_map_zero_or_more_iterator_gen_invariant
+  (#pe: cbor_parser)
+  (#minl: (cbor_min_length pe))
+  (#maxl: (cbor_max_length pe))
+  (p: (cbor_map_parser minl maxl))
+  (#key: typ) (#tkey: Type0)
+  (sp1: (spec key tkey true))
+  (#value: typ) (#tvalue: Type0)
+  (#inj: bool)
+  (sp2: (spec value tvalue inj))
+  (except: map_constraint { inj \/ map_constraint_value_injective key sp2.parser except })
+  (em: bool)
+  (out: S.slice U8.t)
+  (vout: Seq.seq U8.t)
+  (size: SZ.t)
+  (count: U64.t)
+  (m: cbor_map)
+  (v0: Map.t tkey (list tvalue))
+  (v: Map.t tkey (list tvalue))
+  (min: nat)
+  (max: option nat)
+  (res: bool)
+: prop
+= impl_serialize_map_zero_or_more_iterator_gen_invariant1 p sp1 sp2 except em out vout size count m v0 v min max res
