src/cddl/pulse/CDDL.Pulse.Serialize.Gen.MapGroup.ZeroOrMore.Aux2.Proof0.fsti
@@ -16,22 +16,29 @@ module Map = CDDL.Spec.Map
 
 module SM = Pulse.Lib.SeqMatch
 
-val impl_serialize_map_zero_or_more_iterator_gen_invariant_implies_invariant0
+val impl_serialize_map_zero_or_more_iterator_gen_invariant_implies_invariant1
   (#pe: cbor_parser)
   (#minl: (cbor_min_length pe))
   (#maxl: (cbor_max_length pe))
-  (#tkey: Type)
-  (#tvalue: Type)
   (p: (cbor_map_parser minl maxl))
+  (#key: typ) (#tkey: Type0)
+  (sp1: (spec key tkey true))
+  (#value: typ) (#tvalue: Type0)
+  (#inj: bool)
+  (sp2: (spec value tvalue inj))
+  (except: map_constraint { inj \/ map_constraint_value_injective key sp2.parser except })
   (em: bool)
   (out: S.slice U8.t)
   (vout: Seq.seq U8.t)
   (size: SZ.t)
   (count: U64.t)
   (m: cbor_map)
+  (v0: Map.t tkey (list tvalue))
   (v: Map.t tkey (list tvalue))
+  (min: nat)
+  (max: option nat)
   (res: bool)
 : Lemma
-  (requires impl_serialize_map_zero_or_more_iterator_gen_invariant p em out vout size count m v res)
-  (ensures impl_serialize_map_zero_or_more_iterator_gen_invariant0 p em out vout size count m v res)
-  [SMTPat (impl_serialize_map_zero_or_more_iterator_gen_invariant p em out vout size count m v res)]
+  (requires impl_serialize_map_zero_or_more_iterator_gen_invariant p sp1 sp2 except em out vout size count m v0 v min max res)
+  (ensures impl_serialize_map_zero_or_more_iterator_gen_invariant1 p sp1 sp2 except em out vout size count m v0 v min max res)
+  [SMTPat (impl_serialize_map_zero_or_more_iterator_gen_invariant p sp1 sp2 except em out vout size count m v0 v min max res)]
